Updated form of scoped syntax to be parallel to well-typed version

coq/well-scoped-sums/utlc.sig
@@ -1,0 +1,12 @@
+ty : Type
+tm: Type
+
+Base : ty 
+Fun : ty -> ty -> ty
+Plus : ty -> ty -> ty
+
+app : tm -> tm -> tm
+lam : ty -> (tm -> tm) -> tm
+inl : tm -> tm 
+inr : tm -> tm 
+orelim : tm -> (tm -> tm) -> (tm -> tm) -> tm
