coq/well-scoped/utlc.sig
@@ -1,0 +1,8 @@
+ty : Type
+tm: Type
+
+Base : ty 
+Fun : ty -> ty -> ty
+
+app : tm -> tm -> tm
+lam : ty -> (tm -> tm) -> tm
