coq/well-typed/sn.v.d
@@ -1,2 +1,0 @@
-sn.vo sn.glob sn.v.beautified: sn.v ./base.vo ./contexts.vo ./stlc.vo ./reduction.vo
-sn.vio: sn.v ./base.vio ./contexts.vio ./stlc.vio ./reduction.vio
