coq/well-typed/sn_inductive.v.d
@@ -1,2 +1,0 @@
-sn_inductive.vo sn_inductive.glob sn_inductive.v.beautified: sn_inductive.v ./base.vo ./contexts.vo ./stlc.vo ./reduction.vo
-sn_inductive.vio: sn_inductive.v ./base.vio ./contexts.vio ./stlc.vio ./reduction.vio
