coq/well-scoped-sums/stlc.v
@@ -2,7 +2,8 @@ Require Export fintype.
 
 Inductive ty  : Type :=
   | Base : ty 
-  | Fun : ty  -> ty  -> ty .
+  | Fun : ty  -> ty  -> ty 
+  | Plus : ty  -> ty  -> ty .
 
 Lemma congr_Base  : Base  = Base  .
 Proof. congruence. Qed.
@@ -10,15 +11,30 @@ Proof. congruence. Qed.
 Lemma congr_Fun  { s0 : ty  } { s1 : ty  } { t0 : ty  } { t1 : ty  } : s0 = t0 -> s1 = t1 -> Fun s0 s1 = Fun t0 t1 .
 Proof. congruence. Qed.
 
+Lemma congr_Plus  { s0 : ty  } { s1 : ty  } { t0 : ty  } { t1 : ty  } : s0 = t0 -> s1 = t1 -> Plus s0 s1 = Plus t0 t1 .
+Proof. congruence. Qed.
+
 Inductive tm (ntm : nat) : Type :=
   | var_tm : fin (ntm) -> tm (ntm)
   | app : tm (ntm) -> tm (ntm) -> tm (ntm)
-  | lam : ty  -> tm (S ntm) -> tm (ntm).
+  | lam : ty  -> tm (S ntm) -> tm (ntm)
+  | inl : tm (ntm) -> tm (ntm)
+  | inr : tm (ntm) -> tm (ntm)
+  | orelim : tm (ntm) -> tm (S ntm) -> tm (S ntm) -> tm (ntm).
 
 Lemma congr_app { mtm : nat } { s0 : tm (mtm) } { s1 : tm (mtm) } { t0 : tm (mtm) } { t1 : tm (mtm) } : s0 = t0 -> s1 = t1 -> app (mtm) s0 s1 = app (mtm) t0 t1 .
 Proof. congruence. Qed.
 
 Lemma congr_lam { mtm : nat } { s0 : ty  } { s1 : tm (S mtm) } { t0 : ty  } { t1 : tm (S mtm) } : s0 = t0 -> s1 = t1 -> lam (mtm) s0 s1 = lam (mtm) t0 t1 .
+Proof. congruence. Qed.
+
+Lemma congr_inl { mtm : nat } { s0 : tm (mtm) } { t0 : tm (mtm) } : s0 = t0 -> inl (mtm) s0 = inl (mtm) t0 .
+Proof. congruence. Qed.
+
+Lemma congr_inr { mtm : nat } { s0 : tm (mtm) } { t0 : tm (mtm) } : s0 = t0 -> inr (mtm) s0 = inr (mtm) t0 .
+Proof. congruence. Qed.
+
+Lemma congr_orelim { mtm : nat } { s0 : tm (mtm) } { s1 : tm (S mtm) } { s2 : tm (S mtm) } { t0 : tm (mtm) } { t1 : tm (S mtm) } { t2 : tm (S mtm) } : s0 = t0 -> s1 = t1 -> s2 = t2 -> orelim (mtm) s0 s1 s2 = orelim (mtm) t0 t1 t2 .
 Proof. congruence. Qed.
 
 Definition upRen_tm_tm { m : nat } { n : nat } (xi : fin (m) -> fin (n)) : _ :=
@@ -29,6 +45,9 @@ Fixpoint ren_tm { mtm : nat } { ntm : nat } (xitm : fin (mtm) -> fin (ntm)) (s :
     | var_tm (_) s => (var_tm (ntm)) (xitm s)
     | app (_) s0 s1 => app (ntm) (ren_tm xitm s0) (ren_tm xitm s1)
     | lam (_) s0 s1 => lam (ntm) s0 (ren_tm (upRen_tm_tm xitm) s1)
+    | inl (_) s0 => inl (ntm) (ren_tm xitm s0)
+    | inr (_) s0 => inr (ntm) (ren_tm xitm s0)
+    | orelim (_) s0 s1 s2 => orelim (ntm) (ren_tm xitm s0) (ren_tm (upRen_tm_tm xitm) s1) (ren_tm (upRen_tm_tm xitm) s2)
     end.
 
 Definition up_tm_tm { m : nat } { ntm : nat } (sigma : fin (m) -> tm (ntm)) : _ :=
@@ -39,6 +58,9 @@ Fixpoint subst_tm { mtm : nat } { ntm : nat } (sigmatm : fin (mtm) -> tm (ntm)) 
     | var_tm (_) s => sigmatm s
     | app (_) s0 s1 => app (ntm) (subst_tm sigmatm s0) (subst_tm sigmatm s1)
     | lam (_) s0 s1 => lam (ntm) s0 (subst_tm (up_tm_tm sigmatm) s1)
+    | inl (_) s0 => inl (ntm) (subst_tm sigmatm s0)
+    | inr (_) s0 => inr (ntm) (subst_tm sigmatm s0)
+    | orelim (_) s0 s1 s2 => orelim (ntm) (subst_tm sigmatm s0) (subst_tm (up_tm_tm sigmatm) s1) (subst_tm (up_tm_tm sigmatm) s2)
     end.
 
 Definition upId_tm_tm { mtm : nat } (sigma : fin (mtm) -> tm (mtm)) (Eq : forall x, sigma x = (var_tm (mtm)) x) : forall x, (up_tm_tm sigma) x = (var_tm (S mtm)) x :=
@@ -52,6 +74,9 @@ Fixpoint idSubst_tm { mtm : nat } (sigmatm : fin (mtm) -> tm (mtm)) (Eqtm : fora
     | var_tm (_) s => Eqtm s
     | app (_) s0 s1 => congr_app (idSubst_tm sigmatm Eqtm s0) (idSubst_tm sigmatm Eqtm s1)
     | lam (_) s0 s1 => congr_lam (eq_refl s0) (idSubst_tm (up_tm_tm sigmatm) (upId_tm_tm (_) Eqtm) s1)
+    | inl (_) s0 => congr_inl (idSubst_tm sigmatm Eqtm s0)
+    | inr (_) s0 => congr_inr (idSubst_tm sigmatm Eqtm s0)
+    | orelim (_) s0 s1 s2 => congr_orelim (idSubst_tm sigmatm Eqtm s0) (idSubst_tm (up_tm_tm sigmatm) (upId_tm_tm (_) Eqtm) s1) (idSubst_tm (up_tm_tm sigmatm) (upId_tm_tm (_) Eqtm) s2)
     end.
 
 Definition upExtRen_tm_tm { m : nat } { n : nat } (xi : fin (m) -> fin (n)) (zeta : fin (m) -> fin (n)) (Eq : forall x, xi x = zeta x) : forall x, (upRen_tm_tm xi) x = (upRen_tm_tm zeta) x :=
@@ -65,6 +90,9 @@ Fixpoint extRen_tm { mtm : nat } { ntm : nat } (xitm : fin (mtm) -> fin (ntm)) (
     | var_tm (_) s => ap (var_tm (ntm)) (Eqtm s)
     | app (_) s0 s1 => congr_app (extRen_tm xitm zetatm Eqtm s0) (extRen_tm xitm zetatm Eqtm s1)
     | lam (_) s0 s1 => congr_lam (eq_refl s0) (extRen_tm (upRen_tm_tm xitm) (upRen_tm_tm zetatm) (upExtRen_tm_tm (_) (_) Eqtm) s1)
+    | inl (_) s0 => congr_inl (extRen_tm xitm zetatm Eqtm s0)
+    | inr (_) s0 => congr_inr (extRen_tm xitm zetatm Eqtm s0)
+    | orelim (_) s0 s1 s2 => congr_orelim (extRen_tm xitm zetatm Eqtm s0) (extRen_tm (upRen_tm_tm xitm) (upRen_tm_tm zetatm) (upExtRen_tm_tm (_) (_) Eqtm) s1) (extRen_tm (upRen_tm_tm xitm) (upRen_tm_tm zetatm) (upExtRen_tm_tm (_) (_) Eqtm) s2)
     end.
 
 Definition upExt_tm_tm { m : nat } { ntm : nat } (sigma : fin (m) -> tm (ntm)) (tau : fin (m) -> tm (ntm)) (Eq : forall x, sigma x = tau x) : forall x, (up_tm_tm sigma) x = (up_tm_tm tau) x :=
@@ -78,6 +106,9 @@ Fixpoint ext_tm { mtm : nat } { ntm : nat } (sigmatm : fin (mtm) -> tm (ntm)) (t
     | var_tm (_) s => Eqtm s
     | app (_) s0 s1 => congr_app (ext_tm sigmatm tautm Eqtm s0) (ext_tm sigmatm tautm Eqtm s1)
     | lam (_) s0 s1 => congr_lam (eq_refl s0) (ext_tm (up_tm_tm sigmatm) (up_tm_tm tautm) (upExt_tm_tm (_) (_) Eqtm) s1)
+    | inl (_) s0 => congr_inl (ext_tm sigmatm tautm Eqtm s0)
+    | inr (_) s0 => congr_inr (ext_tm sigmatm tautm Eqtm s0)
+    | orelim (_) s0 s1 s2 => congr_orelim (ext_tm sigmatm tautm Eqtm s0) (ext_tm (up_tm_tm sigmatm) (up_tm_tm tautm) (upExt_tm_tm (_) (_) Eqtm) s1) (ext_tm (up_tm_tm sigmatm) (up_tm_tm tautm) (upExt_tm_tm (_) (_) Eqtm) s2)
     end.
 
 Fixpoint compRenRen_tm { ktm : nat } { ltm : nat } { mtm : nat } (xitm : fin (mtm) -> fin (ktm)) (zetatm : fin (ktm) -> fin (ltm)) (rhotm : fin (mtm) -> fin (ltm)) (Eqtm : forall x, (funcomp zetatm xitm) x = rhotm x) (s : tm (mtm)) : ren_tm zetatm (ren_tm xitm s) = ren_tm rhotm s :=
@@ -85,6 +116,9 @@ Fixpoint compRenRen_tm { ktm : nat } { ltm : nat } { mtm : nat } (xitm : fin (mt
     | var_tm (_) s => ap (var_tm (ltm)) (Eqtm s)
     | app (_) s0 s1 => congr_app (compRenRen_tm xitm zetatm rhotm Eqtm s0) (compRenRen_tm xitm zetatm rhotm Eqtm s1)
     | lam (_) s0 s1 => congr_lam (eq_refl s0) (compRenRen_tm (upRen_tm_tm xitm) (upRen_tm_tm zetatm) (upRen_tm_tm rhotm) (up_ren_ren (_) (_) (_) Eqtm) s1)
+    | inl (_) s0 => congr_inl (compRenRen_tm xitm zetatm rhotm Eqtm s0)
+    | inr (_) s0 => congr_inr (compRenRen_tm xitm zetatm rhotm Eqtm s0)
+    | orelim (_) s0 s1 s2 => congr_orelim (compRenRen_tm xitm zetatm rhotm Eqtm s0) (compRenRen_tm (upRen_tm_tm xitm) (upRen_tm_tm zetatm) (upRen_tm_tm rhotm) (up_ren_ren (_) (_) (_) Eqtm) s1) (compRenRen_tm (upRen_tm_tm xitm) (upRen_tm_tm zetatm) (upRen_tm_tm rhotm) (up_ren_ren (_) (_) (_) Eqtm) s2)
     end.
 
 Definition up_ren_subst_tm_tm { k : nat } { l : nat } { mtm : nat } (xi : fin (k) -> fin (l)) (tau : fin (l) -> tm (mtm)) (theta : fin (k) -> tm (mtm)) (Eq : forall x, (funcomp tau xi) x = theta x) : forall x, (funcomp (up_tm_tm tau) (upRen_tm_tm xi)) x = (up_tm_tm theta) x :=
@@ -98,6 +132,9 @@ Fixpoint compRenSubst_tm { ktm : nat } { ltm : nat } { mtm : nat } (xitm : fin (
     | var_tm (_) s => Eqtm s
     | app (_) s0 s1 => congr_app (compRenSubst_tm xitm tautm thetatm Eqtm s0) (compRenSubst_tm xitm tautm thetatm Eqtm s1)
     | lam (_) s0 s1 => congr_lam (eq_refl s0) (compRenSubst_tm (upRen_tm_tm xitm) (up_tm_tm tautm) (up_tm_tm thetatm) (up_ren_subst_tm_tm (_) (_) (_) Eqtm) s1)
+    | inl (_) s0 => congr_inl (compRenSubst_tm xitm tautm thetatm Eqtm s0)
+    | inr (_) s0 => congr_inr (compRenSubst_tm xitm tautm thetatm Eqtm s0)
+    | orelim (_) s0 s1 s2 => congr_orelim (compRenSubst_tm xitm tautm thetatm Eqtm s0) (compRenSubst_tm (upRen_tm_tm xitm) (up_tm_tm tautm) (up_tm_tm thetatm) (up_ren_subst_tm_tm (_) (_) (_) Eqtm) s1) (compRenSubst_tm (upRen_tm_tm xitm) (up_tm_tm tautm) (up_tm_tm thetatm) (up_ren_subst_tm_tm (_) (_) (_) Eqtm) s2)
     end.
 
 Definition up_subst_ren_tm_tm { k : nat } { ltm : nat } { mtm : nat } (sigma : fin (k) -> tm (ltm)) (zetatm : fin (ltm) -> fin (mtm)) (theta : fin (k) -> tm (mtm)) (Eq : forall x, (funcomp (ren_tm zetatm) sigma) x = theta x) : forall x, (funcomp (ren_tm (upRen_tm_tm zetatm)) (up_tm_tm sigma)) x = (up_tm_tm theta) x :=
@@ -111,6 +148,9 @@ Fixpoint compSubstRen__tm { ktm : nat } { ltm : nat } { mtm : nat } (sigmatm : f
     | var_tm (_) s => Eqtm s
     | app (_) s0 s1 => congr_app (compSubstRen__tm sigmatm zetatm thetatm Eqtm s0) (compSubstRen__tm sigmatm zetatm thetatm Eqtm s1)
     | lam (_) s0 s1 => congr_lam (eq_refl s0) (compSubstRen__tm (up_tm_tm sigmatm) (upRen_tm_tm zetatm) (up_tm_tm thetatm) (up_subst_ren_tm_tm (_) (_) (_) Eqtm) s1)
+    | inl (_) s0 => congr_inl (compSubstRen__tm sigmatm zetatm thetatm Eqtm s0)
+    | inr (_) s0 => congr_inr (compSubstRen__tm sigmatm zetatm thetatm Eqtm s0)
+    | orelim (_) s0 s1 s2 => congr_orelim (compSubstRen__tm sigmatm zetatm thetatm Eqtm s0) (compSubstRen__tm (up_tm_tm sigmatm) (upRen_tm_tm zetatm) (up_tm_tm thetatm) (up_subst_ren_tm_tm (_) (_) (_) Eqtm) s1) (compSubstRen__tm (up_tm_tm sigmatm) (upRen_tm_tm zetatm) (up_tm_tm thetatm) (up_subst_ren_tm_tm (_) (_) (_) Eqtm) s2)
     end.
 
 Definition up_subst_subst_tm_tm { k : nat } { ltm : nat } { mtm : nat } (sigma : fin (k) -> tm (ltm)) (tautm : fin (ltm) -> tm (mtm)) (theta : fin (k) -> tm (mtm)) (Eq : forall x, (funcomp (subst_tm tautm) sigma) x = theta x) : forall x, (funcomp (subst_tm (up_tm_tm tautm)) (up_tm_tm sigma)) x = (up_tm_tm theta) x :=
@@ -124,6 +164,9 @@ Fixpoint compSubstSubst_tm { ktm : nat } { ltm : nat } { mtm : nat } (sigmatm : 
     | var_tm (_) s => Eqtm s
     | app (_) s0 s1 => congr_app (compSubstSubst_tm sigmatm tautm thetatm Eqtm s0) (compSubstSubst_tm sigmatm tautm thetatm Eqtm s1)
     | lam (_) s0 s1 => congr_lam (eq_refl s0) (compSubstSubst_tm (up_tm_tm sigmatm) (up_tm_tm tautm) (up_tm_tm thetatm) (up_subst_subst_tm_tm (_) (_) (_) Eqtm) s1)
+    | inl (_) s0 => congr_inl (compSubstSubst_tm sigmatm tautm thetatm Eqtm s0)
+    | inr (_) s0 => congr_inr (compSubstSubst_tm sigmatm tautm thetatm Eqtm s0)
+    | orelim (_) s0 s1 s2 => congr_orelim (compSubstSubst_tm sigmatm tautm thetatm Eqtm s0) (compSubstSubst_tm (up_tm_tm sigmatm) (up_tm_tm tautm) (up_tm_tm thetatm) (up_subst_subst_tm_tm (_) (_) (_) Eqtm) s1) (compSubstSubst_tm (up_tm_tm sigmatm) (up_tm_tm tautm) (up_tm_tm thetatm) (up_subst_subst_tm_tm (_) (_) (_) Eqtm) s2)
     end.
 
 Definition rinstInst_up_tm_tm { m : nat } { ntm : nat } (xi : fin (m) -> fin (ntm)) (sigma : fin (m) -> tm (ntm)) (Eq : forall x, (funcomp (var_tm (ntm)) xi) x = sigma x) : forall x, (funcomp (var_tm (S ntm)) (upRen_tm_tm xi)) x = (up_tm_tm sigma) x :=
@@ -137,6 +180,9 @@ Fixpoint rinst_inst_tm { mtm : nat } { ntm : nat } (xitm : fin (mtm) -> fin (ntm
     | var_tm (_) s => Eqtm s
     | app (_) s0 s1 => congr_app (rinst_inst_tm xitm sigmatm Eqtm s0) (rinst_inst_tm xitm sigmatm Eqtm s1)
     | lam (_) s0 s1 => congr_lam (eq_refl s0) (rinst_inst_tm (upRen_tm_tm xitm) (up_tm_tm sigmatm) (rinstInst_up_tm_tm (_) (_) Eqtm) s1)
+    | inl (_) s0 => congr_inl (rinst_inst_tm xitm sigmatm Eqtm s0)
+    | inr (_) s0 => congr_inr (rinst_inst_tm xitm sigmatm Eqtm s0)
+    | orelim (_) s0 s1 s2 => congr_orelim (rinst_inst_tm xitm sigmatm Eqtm s0) (rinst_inst_tm (upRen_tm_tm xitm) (up_tm_tm sigmatm) (rinstInst_up_tm_tm (_) (_) Eqtm) s1) (rinst_inst_tm (upRen_tm_tm xitm) (up_tm_tm sigmatm) (rinstInst_up_tm_tm (_) (_) Eqtm) s2)
     end.
 
 Lemma rinstInst_tm { mtm : nat } { ntm : nat } (xitm : fin (mtm) -> fin (ntm)) : ren_tm xitm = subst_tm (funcomp (var_tm (ntm)) xitm) .
@@ -183,6 +229,12 @@ Arguments var_tm {ntm}.
 Arguments app {ntm}.
 
 Arguments lam {ntm}.
+
+Arguments inl {ntm}.
+
+Arguments inr {ntm}.
+
+Arguments orelim {ntm}.
 
 Instance Subst_tm { mtm : nat } { ntm : nat } : Subst1 (fin (mtm) -> tm (ntm)) (tm (mtm)) (tm (ntm)) := @subst_tm (mtm) (ntm) .
 
