coq/well-scoped/sn.v
@@ -1,311 +1,106 @@
-(** * Proof of Strong Normalisation *)
+Require Import base contexts stlc reduction.
 
-Require Import axioms fintype stlc ARS.
-Set Implicit Arguments.
-Unset Strict Implicit.
+(** ** Logical Relation *)
 
-Ltac inv H := inversion H; subst; clear H.
-Notation "M .[ sigma ]'" := (ren_tm sigma M) (at level 60, format "M .[ sigma ]'").
-Notation "M .[ sigma ]" := (subst_tm sigma M) (at level 60, format "M .[ sigma ]").
-
-(** ** One-Step Reduction *)
-Inductive step {n} : tm n -> tm n -> Prop :=
-| step_beta (T : ty) (M : tm (S n)) (N : tm n) :
-    step (app (lam T M) N) (M.[N .: var_tm])
-| step_appL M N M' :
-    step M M' -> step (app M N) (app M' N)
-| step_appR M N N' :
-    step N N' -> step (app M N) (app M N')
-| step_abs T M M' :
-    @step (S n) M M' -> step (lam T M) (lam T M').
-
-Lemma step_ebeta {n} T M N (M' : tm n) :
-  M' = M.[N .: var_tm] -> step (app (lam T M) N) M'.
-Proof. intros ->. apply step_beta. Qed.
-
-Module Reduction.
-Lemma substitutivity {n1 n2} (sigma : fin n1 -> tm n2) M M' :
-  step M M' -> step (M.[sigma]) (M'.[sigma]).
-Proof.
-  intros H. revert n2 sigma. induction H; intros n2 sigma; asimpl; eauto using @step.
-  - apply step_ebeta. now asimpl.
-Qed.
-
-Lemma naturality m n (M: tm m) (rho: fin m -> fin n) N :
-  step (M.[rho]') N -> exists N', step M N' /\ N = (ren_tm rho N').
-Proof.
-  revert n N rho. induction M as [m x | m M1 IHM1 M2 IHM2 | m T M IHM]; intros n N rho H.
-  - inv H.
-  - inv H.
-    + assert (exists s1', M1 = lam T s1' ) as [s1' B].
-      { destruct M1; simpl in *; try congruence; eauto. inversion H1. subst. eauto. }
-      subst.
-      exists (s1'.[M2 .: var_tm]). split.
-      * constructor.
-      * revert H1. asimpl. intros H1. inv H1. asimpl. reflexivity.
-    + destruct (IHM1 _ _ _ H3) as (M1'&IH11&IH12). subst.
-      exists (app M1' M2). split. constructor. assumption.
-      reflexivity.
-    + destruct (IHM2 _ _ _ H3) as (M2'&IH21&IH22).
-      subst. exists (app M1 M2').  split. now constructor. reflexivity.
-  - inv H.
-    destruct (IHM _ _ _ H3) as (N'&IH1&->).
-    exists (lam T N'). split. now apply step_abs. reflexivity.
-Qed.
-
-End Reduction.
-
-(** ** Many-Step Reduction *)
-Definition red {n} := star (@step n).
-
-Definition sred {n k} (sigma tau : fin n -> tm k) :=
-  forall x, @red k (sigma x) (tau x).
-
-Module ManyStepReduction.
-Lemma red_app {n} (M M' N N' : tm n) :
-  red M M' -> red N N' -> red (app M N) (app M' N').
-Proof.
-  intros T B. apply (star_trans (app M' N)).
-  - eapply (star_hom (fun M => @app n M N)); [|eauto].
-    + intros. eapply step_appL; exact H.
-  - eapply star_hom; [|eauto]. eauto using step_appR.
-Qed.
-
-Lemma red_abs {n} T (M M' : tm (S n)) :
-  red M M' -> red (lam T M) (lam T M').
-Proof. apply star_hom. eauto using step_abs. Qed.
-
-Lemma red_inst {n1 n2} (f : fin n1 -> tm n2) s t :
-  red s t -> red (s.[f]) (t.[f]).
-Proof. apply star_hom. eauto using Reduction.substitutivity. Qed.
-
-Lemma red_compat {n1 n2} (f1 f2 : fin n1 -> tm n2) s :
-  sred f1 f2 -> red (s.[f1]) (s.[f2]).
-Proof.
-  revert n2 f1 f2; induction s; intros n2 f1 f2 H; asimpl; eauto using red_app, red_abs.
-  - apply red_abs, IHs. intros [i|]; [|constructor].
-    apply red_inst, H.
-Qed.
-
-Lemma red_beta {n} s (N N' : tm n) :
-  step N N' -> red (s.[N .: var_tm]) (s.[N' .: var_tm]).
-Proof. intros h. apply red_compat. intros [i|]; [now apply starR|now apply star1]. Qed.
-
-End ManyStepReduction.
-Import ManyStepReduction.
-
-(** ** Strong Normalisation *)
-Notation sn := (sn (@step _)).
-Module SN.
-Lemma closed_app {n} (t s : tm n) :
-  sn (app s t) -> sn s.
-Proof. apply (sn_preimage (h := fun M => @app n M t)). eauto using step_appL. Qed.
-
-Lemma substitutivity {n1 n2} (f : fin n1 -> tm n2) s :
-  sn (s.[f]) -> sn s.
-Proof. apply sn_preimage. apply Reduction.substitutivity. Qed.
-
-(** *** Lemma 2.4 - SN Closure under Weakening *)
-Lemma weak k (M: tm k) k' (rho : fin k -> fin k'):
-  sn M -> sn (M .[rho]').
-Proof.
-  intros H. revert k' rho. induction H as [x H IH]; intros k' rho.
-  apply SNI. intros x' A.
-  destruct (Reduction.naturality A) as (x''&B1&B2); subst.
-  now apply IH.
-Qed.
-End SN.
-
-(** ** Syntactic typing *)
-Definition ctx n := fin n -> ty.
-Inductive has_type {n} (Gamma : ctx n) : tm n -> ty -> Prop :=
-| ty_var_tm (x : fin n) :
-    has_type Gamma (var_tm x) (Gamma x)
-| ty_abs (S1 S2 : ty) (M : tm (S n)) :
-    @has_type (S n) (S1 .: Gamma) M S2 ->
-    has_type Gamma (lam S1 M) (arr S1 S2)
-| ty_app (T S : ty) (M N : tm n) :
-    has_type Gamma M (arr T S) ->
-    has_type Gamma N T ->
-    has_type Gamma (app M N) S.
-Notation "Gamma |- M : T" := (has_type Gamma M T) (at level 20, M at level 99).
-Definition ltc {k k'} (Gamma: ctx k) (Delta: ctx k') rho := forall x, Delta (rho x) = Gamma x.
-
-Module Typing.
-Lemma typing_ren n k (Gamma: ctx n) (Delta: ctx k) (rho: fin n -> fin k) (M: tm n) T :
-  ltc Gamma Delta rho  -> Gamma |- M : T ->  Delta |- (M .[rho]') : T.
-Proof.
-  intros H B. revert k rho Delta H. induction B as [x | n Gamma T1 T2 M A IH | n Gamma T1 T2 M N A IHA B IHB]; intros k rho Delta H.
-  - rewrite <- H. apply ty_var_tm.
-  - apply ty_abs. apply IH.
-    intros [x|]; [|constructor]. asimpl. apply H.
-  - eapply ty_app; eauto.
-Qed.
-
-Lemma typing_inst n k (Gamma: ctx n) (Delta: ctx k) (sigma: fin n -> tm k) (M: tm n) T :
-  (forall x, Delta |- sigma x : Gamma x) -> Gamma |- M : T ->  Delta |- (M.[sigma]) : T.
-Proof.
-  intros A B. revert k sigma Delta A.  induction B as [x | n Gamma T1 T2 M A IH | n Gamma T1 T2 M N A IHA B IHB]; intros k sigma Delta H.
-  - apply H.
-  - apply ty_abs. apply IH.
-    intros [x|]; [|constructor]. eapply typing_ren; [intros y; reflexivity|apply H].
-  - apply ty_app with (T := T1); eauto.
-Qed.
-
-Lemma step_typing k (Gamma: ctx k) M T :
-  Gamma |- M : T -> forall M', step M M' -> Gamma |- M' : T.
-Proof.
-  induction 1 as [k Gamma x | k Gamma T S M A IHA | k Gamma T S M N A IHA B IHB]; intros M' H; cbn.
-  - inv H.
-  - inv H. econstructor. now apply IHA.
-  - inv H.
-    + inv A. eapply typing_inst; try eassumption.
-      intros [i|]; [econstructor | assumption].
-    + eapply ty_app. now apply IHA. assumption.
-    + eapply ty_app.
-      * exact A.
-      * now apply IHB.
-Qed.
-End Typing.
-Import Typing.
-
-
-(** ** The Reducibility Candidates/Logical Predicate*)
-Definition cand n := tm n -> Prop.
-
-Fixpoint L {k} (Gamma: ctx k) (T: ty) : cand k :=
-  match T with
-  |Base => fun M => Gamma |- M : T /\ sn M
-  |arr T1 T2 => fun M => Gamma |- M : arr T1 T2 /\
-                     (forall k' (N: tm k') (Delta: ctx k') rho, ltc Gamma Delta rho -> L Delta T1 N -> L Delta T2 (app (M.[rho]') N))
+Fixpoint L (G : ctx) (A : ty) : tm G A -> Prop :=
+  match A with
+  | Base => sn
+  | Fun A B => fun s =>
+      forall G' (f : ren G G') (t : tm G' A), L t -> L (app (rinst f s) t)
   end.
 
-Lemma L_typing {k} (Gamma: ctx k) (T: ty) M :
-  L Gamma T M -> Gamma |- M : T.
-Proof. intros H. destruct T; simpl in *; intuition. Qed.
+(** Lemma 10 *)
 
-Module L.
-
-Lemma preservation {k} (Gamma : ctx k) M M' T :
-  step M M' -> L Gamma T M -> L Gamma T M'.
+Lemma L_step G A (s t : tm G A) :
+  step s t -> L s -> L t.
 Proof.
-  revert k Gamma M M'. induction T as [|T IHT S IHS]; intros k Gamma M M' M_M' [H1 H2].
-  - split.
-    + eapply step_typing; eassumption.
-    + inv H2. now apply H.
-  - split; [|].
-    + eapply step_typing; eassumption.
-    + intros k' N Delta rho H H0. apply IHS with (M := app (M.[rho]') N).
-      * econstructor. asimpl. now apply Reduction.substitutivity.
-      * now apply H2.
+  elim: A G s t => /=[G s t st [H]|A ih1 B ih2 G1 s t st ls G2 f u lu]. exact: H.
+  apply: ih2; last by exact: ls lu. apply: step_appL. rewrite !rinst_inst. exact: step_inst.
 Qed.
 
-Lemma preservation_red {k} (Gamma : ctx k) M M' T :
-  red M M' -> L Gamma T M -> L Gamma T M'.
-Proof. intros H. induction H; eauto using preservation. Qed.
-
-Lemma ren k k' (Gamma: ctx k) (Delta: ctx k') rho M T (Gamma_Delta : ltc Gamma Delta rho):
-  L Gamma T M -> L Delta T (M .[rho]').
+Lemma L_mstep G A (s t : tm G A) :
+  mstep s t -> L s -> L t.
 Proof.
-  induction T as [|T IHT S IHS]; intros [H1 H2]; split; try apply typing_ren with (Gamma := Gamma); eauto.
-  - now apply SN.weak.
-  - intros k'' N Delta' rho' A1 A2.
-    assert ((M.[rho]').[rho']' = M.[rho >> rho']') as -> by (now asimpl).
-    apply H2; [|assumption].
-    + intros x. now rewrite <- Gamma_Delta, <- A1.
+  elim=>//{t}t u _ ih /L_step; tauto.
 Qed.
 
-Definition neutral k (M: tm k) :=
-  match M with
-  |lam _ _ => False
-  |_ => True
-  end.
+(** Lemma 11 *)
 
-(** Girard's theorem. *)
-Lemma Girard k (Gamma: ctx k) (M : tm k) T :
-  (L Gamma T M -> sn M) /\ (Gamma |- M : T -> neutral M -> (forall N, step M N -> L Gamma T N) -> L Gamma T M).
+Lemma L_rinst G1 G2 A (f : ren G1 G2) (s : tm G1 A) :
+  L s -> L (rinst f s).
 Proof.
-  revert k M Gamma. induction T as [|T1 IHT1 T2 IHT2]; intros k M Gamma; simpl in *.
-  - intuition. constructor. intros N H'. firstorder.
-  - split.
-    + intros [H1 H2].
-      assert (A:  L (T1 .: Gamma) T2 (app (M .[shift]') (@var_tm (S k) None))).
-      { apply H2. intros x; reflexivity. apply IHT1. constructor. constructor. intros N H. inv H. }
-      erewrite rinst_inst_tm in A; [|reflexivity].
-      now eapply IHT2, SN.closed_app, SN.substitutivity in A.
-     + intros H0 H1 H2. split; [assumption |].
-      intros k' N Delta rho H3 H4.
-      assert ( SN_N : sn N) by firstorder.
-      induction SN_N as [N sn_N IHN].
-      apply IHT2; try constructor.
-       * erewrite rinst_inst_tm; [|reflexivity]. eapply ty_app.
-         -- eapply typing_inst; try eassumption.
-            intros x. rewrite <- H3. constructor.
-         -- auto using L_typing.
-      * intros M' A. inv A.
-        -- destruct M; simpl in *; try congruence. contradiction.
-        -- destruct (Reduction.naturality H7) as [M'' [H' ->]]. now apply H2.
-        -- apply IHN; [assumption|]. eapply preservation; eassumption.
+  case: A s => [|A B] s /=. exact: sn_rinst.
+  move=> H G3 g t lt. rewrite rinst_comp. exact: H.
 Qed.
 
-Lemma sn k (Gamma: ctx k) (M : tm k) T:
-  L Gamma T M -> sn M.
+(** Lemma 12 *)
+
+Definition neutral {G A} (s : tm G A) : bool :=
+  if s is lam _ _ _ then false else true.
+
+Definition neutral_expansion_closed {G A} (P : tm G A -> Prop) :=
+  forall s, neutral s -> (forall t, step s t -> P t) -> P s.
+
+Lemma neutral_expansion_closed_var {G A} P (i : at_ty G A) :
+  neutral_expansion_closed P -> P (var i).
+Proof. apply=> //t st. by inv st. Qed.
+
+Lemma L_sn_nec G A :
+  (forall s : tm G A, L s -> sn s) /\ neutral_expansion_closed (@L G A).
 Proof.
-  intros H. eapply Girard. eassumption.
+  elim: A G => [|A ihA B ihB] G. by split. split.
+  - move=> s /=/(_ (A :: G) shift (var var0)). case/(_ _)/Wrap.
+    apply: neutral_expansion_closed_var. by case: (ihA (A::G)).
+    case: (ihB (A::G)) => h _ /h/sn_appL. by rewrite rinst_inst => /sn_inst.
+  - move=> s ns /=ihs G' f t lt. have snt: sn t. case: (ihA G') => h _. exact: h.
+    elim: snt lt => /={t} t _ iht lt.
+    case: (ihB G') => _ h; apply: h => // u st. inv st.
+    + by inv s.
+    + move: st => /step_weak[s' st <-{s2}]. exact: (ihs s' st).
+    + apply: iht => //. exact: L_step st lt.
 Qed.
 
-Lemma var_tm k (Gamma: ctx k) x :
-  L Gamma (Gamma x) (var_tm x).
-Proof. apply Girard; try constructor. intros N H. inv H. Qed.
+Corollary L_sn G A (s : tm G A) : L s -> sn s.
+Proof. case: (L_sn_nec G A) => H _. exact: H. Qed.
 
-End L.
+Corollary L_nec G A : neutral_expansion_closed (@L G A).
+Proof. by case: (L_sn_nec G A). Qed.
 
-(** ** Closure under beta expansion and the fundamental theorem *)
+Corollary L_var G A (i : at_ty G A) : L (var i).
+Proof. apply: neutral_expansion_closed_var. exact: L_nec. Qed.
 
-Module StrongNormalisation.
+(** Lemma 13 *)
 
-Lemma beta_closure k Gamma (N: tm k) T (N_ty : Gamma |- N : T) :
-  sn N -> forall S M, (T .: Gamma) |- M : S ->  L Gamma S (M.[N .: var_tm]) -> L Gamma S (app (lam T M) N).
+Lemma beta_expansion G A B (s : tm (A :: G) B) t :
+  sn t -> L (inst (t .: ids) s) -> L (app (lam s) t).
 Proof.
-  induction 1 as [N H IH_N]. intros S M M_ty H'.
-  assert (sn_M := SN.substitutivity (L.sn H')). induction sn_M as [M sn_M IH_M].
-  apply L.Girard; try constructor.
-  - now repeat econstructor.
-  - intros M' H1. inv H1; try eauto.
-    + inv H4. apply IH_M; eauto using step_typing, L.preservation, Reduction.substitutivity.
-    + apply IH_N; eauto using step_typing, L.preservation_red, red_beta.
+  move=> snt ls. have sns: sn s. by move: ls => /L_sn/sn_inst.
+  elim: sns t snt ls => {s}s _ ihs t. elim=>{t}t snt iht ls.
+  apply: L_nec => // u st. inv st.
+  - exact: ls.
+  - inv st. apply: ihs. exact: st. constructor. exact: snt.
+    apply: L_step ls. exact: step_inst.
+  - apply: iht. exact: st. apply: L_mstep ls.
+    apply: mstep_beta; eauto using @mstep.
 Qed.
 
-Theorem fundamental_theorem k (Gamma: ctx k) M T :
-  Gamma |- M : T -> forall k' (Gamma': ctx k') sigma,  (forall x,  L Gamma' (Gamma x) (sigma x)) -> L Gamma' T (M.[sigma]).
+Theorem fundamental G1 A (s : tm G1 A) :
+  forall G2 (f : subst G1 G2), (forall B i, L (f B i)) -> L (inst f s).
 Proof.
-  induction 1 as [| k Gamma T1 T2 M H IH | k Gamma T1 T2 M N A IHA B IHB]; intros k' Gamma' sigma adm; asimpl.
-  - apply adm.
-  - assert ( M_ty :  (T1 .: Gamma') |- (M.[@var_tm (S k') bound .: sigma >> ren_tm shift]) : T2).
-    { assert (A: forall x, Gamma' |- sigma x : Gamma x) by auto using L_typing.
-      apply typing_inst with (Gamma := T1 .: Gamma); [|assumption].
-      intros [i|]; [|constructor].
-      -  apply typing_ren with (Gamma := Gamma'); try constructor. apply A. }
-    split.
-    + apply ty_abs. revert M_ty. asimpl. auto.
-    + intros k'0 N Delta rho A B.
-      apply beta_closure; eauto using L_typing, L.sn.
-      * apply typing_ren with (Gamma := T1 .: Gamma'); [intros [i|]; simpl; congruence | ]. revert M_ty. now asimpl.
-      * asimpl. apply IH.
-        intros [i|]; [|assumption].
-        -- unfold up_ren. fsimpl. simpl. unfold funcomp. erewrite <- rinst_inst_tm; [|reflexivity].
-           eapply L.ren. apply A. apply adm.
-  - destruct (IHA _ _ _ adm) as [IHA1 IHA2]. specialize (IHB _ _ _ adm).
-    assert ((M.[sigma]) = ((M.[sigma]).[idren]')) as -> by now asimpl.
-    apply IHA2; unfold ltc; auto.
+  elim: s => {G1 A}[G1 A i|G1 A B s ihs t iht|G1 A B b ih] G2 f fP /=.
+  - exact: fP.
+  - move: (ihs G2 f fP) => /=/(_ G2 idren (inst f t)). rewrite rinst_idren. apply.
+    exact: iht.
+  - move=> G3 g t lt. apply: beta_expansion. exact: L_sn.
+    rewrite rinst_inst_comp inst_comp. apply: ih => C/=[E|i].
+    destruct E => //. cbn. rewrite inst_rinst_comp. fsimpl.
+    rewrite inst_rinst_comp. fsimpl. rewrite -rinst_inst.
+    apply: L_rinst. exact: fP.
 Qed.
 
-
-Corollary strong_normalisation k (Gamma: ctx k) M T :
-  Gamma |- M : T -> sn M.
+Corollary strong_normalization G A (s : tm G A) : sn s.
 Proof.
-  intros A. apply L.sn with (Gamma := Gamma) (T := T).
-  enough (H: L Gamma T  (M.[var_tm])) by now (revert H; asimpl).
-  apply fundamental_theorem with (Gamma := Gamma); auto using L.var_tm.
+  apply: L_sn. move: (@fundamental G A s G ids).
+  case/(_ _)/Wrap. move=> B i. exact: L_var.
+    by rewrite inst_ids.
 Qed.
-End StrongNormalisation.
