coq/well-scoped-sums/contexts.v
@@ -1,0 +1,61 @@
+Require Import base.
+Require Export Lists.List.
+
+(** ** Types *)
+Inductive ty := Base | Fun (A B : ty) | Plus (A B: ty).
+Definition ctx := list ty.
+
+Fixpoint at_ty (G : ctx) (A : ty) : Type :=
+  match G with
+  | nil => False
+  | (B :: G') => (A = B) + at_ty G' A
+  end.
+
+(** ** Environment structure *)
+Definition env (G : ctx) (T : ty -> Type) := forall A, at_ty G A -> T A.
+Definition ren (G1 G2 : ctx) := env G1 (at_ty G2).
+
+Definition scons {G : ctx} {P : ty -> Type} {A : ty} (hd : P A) (tl : env G P) : env (A :: G) P :=
+  fun B i =>
+    match i with
+    | inl p => eq_rect_r P hd p
+    | inr j => tl B j
+    end.
+Notation "hd .: tl" := (@scons _ _ _ hd tl) (at level 55).
+
+Definition scomp {P Q R : ty -> Type} (f : forall A, P A -> Q A) (g : forall A, Q A -> R A) :
+  forall A, P A -> R A := fun A x => g A (f A x).
+Notation "eta >> eps" := (scomp eta eps) (at level 40).
+
+Definition var0 {G : ctx} {A : ty} : at_ty (A :: G) A := inl eq_refl.
+Definition shift {G : ctx} {B : ty} : ren G (B :: G) :=
+  fun A i => inr i.
+
+Definition idren {G : ctx} : ren G G := fun A i => i.
+
+(** ** Environment simplification *)
+Lemma scons_eta G P A (f : env (A :: G) P) : f A var0 .: shift >> f = f.
+Proof. fext. intros B [->|]; auto. Qed.
+
+Lemma scons_eta_id G A : var0 .: shift = @idren (A :: G).
+Proof. fext. intros B [->|]; auto. Qed.
+
+Lemma scons_comp G P Q A (x : P A) (f : env G P) (g : forall A, P A -> Q A) : (x .: f) >> g = (g A x) .: f >> g.
+Proof. fext. intros B [->|]; auto. Qed.
+
+Ltac fsimpl :=
+  repeat match goal with
+    | [|- context[idren >> ?f]] => change (idren >> f) with f
+    | [|- context[?f >> idren]] => change (f >> idren) with f
+    | [|- context[(?f >> ?g) >> ?h]] =>
+        change ((f >> g) >> h) with (f >> (g >> h))
+    | [|- context[@scons ?G ?P ?A ?x ?tl ?B var0]] =>
+      change (@scons G P A x tl B var0) with x
+    | [|- context[shift >> (?x1 .: ?xr)]] =>
+        change (shift >> (x1 .: xr)) with xr
+    | [|- context[?x2 .: shift >> ?f]] =>
+        change x2 with (f _ var0); rewrite (@scons_eta _ _ _ f)
+    | [|- context[?f _ var0 .: ?g]] =>
+        change g with (shift >> f); rewrite scons_eta
+    | _ => first [progress (rewrite scons_comp) | progress (rewrite scons_eta_id)]
+  end.
