coq/well-scoped-sums/reduction.v
@@ -1,0 +1,154 @@
+Require Import stlc Coq.Program.Equality.
+
+(** ** Single-step reduction *)
+Inductive step {n} : tm n -> tm n -> Prop :=
+| step_beta A b t : step (app (lam A b) t) (b[t..])
+| step_abs A b1 b2 : @step (S n) b1 b2 -> step (lam A b1) (lam A b2)
+| step_appL s1 s2 t : step s1 s2 -> step (app s1 t) (app s2 t)
+| step_appR s t1 t2 : step t1 t2 -> step (app s t1) (app s t2)
+| step_inl (s1 s2: tm n) :
+    step s1 s2 -> step (inl s1) (inl s2)
+| step_inr (s1 s2: tm n) :
+    step s1 s2 -> step (inr s1) (inr s2)
+| step_orelim (s1 s2: tm n) (t: tm (S n)) u : step s1 s2 -> step (orelim s1 t u) (orelim s2 t u)
+| step_orelimL  (s: tm n) (t1 t2: tm (S n)) u : @step (S n) t1 t2 -> step (orelim s t1 u) (orelim s t2 u)
+| step_orelimR (s: tm n) (t: tm (S n)) u1 u2 : @step (S n) u1 u2 -> step (orelim s t u1) (orelim s t u2)
+| step_caseL (s: tm n) t (u: tm (S n)) : step (orelim (inl s) t u) (t[s..])
+| step_caseR (s: tm n) (t: tm (S n)) u: step (orelim (inr s) t u) (u[s..])
+.
+
+Lemma step_beta' n A b (t t': tm n):
+  t' = b[t..] -> step (app (lam A b) t) t'.
+Proof. intros ->. now constructor. Qed.
+
+Lemma step_caseL' n  s (t: tm (S n)) t' u:
+  t' = t[s..] -> step (orelim (inl s) t u) t'.
+Proof. intros ->. now constructor. Qed.
+
+Lemma step_caseR' n  s (t: tm (S n))  u u':
+  u' = u[s..] -> step (orelim (inr s) t u) u'.
+Proof. intros ->. now constructor. Qed.
+
+Definition ImPred {T1 T2} (P : T1 -> Prop) (f : T1 -> T2) (y : T2) :=  exists2 x : T1, P x & f x = y.
+
+Notation "[ 'Pred' s | x 'in' P ]" :=
+  (ImPred (fun x => P) (fun x => s)).
+Notation "x ∈ P" := (P x) (at level 30, only parsing).
+
+Ltac inv H := dependent destruction H.
+
+Lemma im_predI {T1 T2} (P : T1 -> Prop) (f : T1 -> T2) (x : T1) :
+  P x -> f x ∈ [Pred f x' | x' in P x'].
+Proof. intros px. now exists x. Qed.
+
+Lemma step_weak {m n} (f : fin m -> fin n) (s : tm m) (t : tm n) :
+  step (s⟨f⟩) t -> t ∈ [Pred ren_tm f s' | s' in step s s'].
+Proof with cbn in *; try congruence.
+  intros st. dependent induction st.
+  - inv s... inv s1; try inv x... asimpl.
+    eexists. constructor. now asimpl.
+  - inv s... inv x. destruct (IHst _ _ _ eq_refl) as [s' ih <-].
+    exists (lam t s'). now constructor. now asimpl.
+  - inv s... inv x. destruct (IHst _ _ _ eq_refl) as [s' ih <-].
+    exists (app s' s4). now constructor. now asimpl.
+  - inv s... inv x. destruct (IHst _ _ _ eq_refl) as [s' ih <-].
+    exists (app s1 s'). now constructor. now asimpl.
+  - inv s... inv x. destruct (IHst _ _ _ eq_refl) as [s' ih <-].
+    exists (inl s'). now constructor. now fsimpl.
+  - inv s... inv x. destruct (IHst _ _ _ eq_refl) as [s' ih <-].
+    exists (inr s'). now constructor. now fsimpl.
+  - inv s... inv x. destruct (IHst _ _ _ eq_refl) as [s' ih <-].
+    exists (orelim s' s4 s5). now constructor. now fsimpl.
+  - inv s... inv x. destruct (IHst _ _ _ eq_refl) as [s' ih <-].
+    exists (orelim s1 s' s3). now constructor. now fsimpl.
+  - inv s... inv x. destruct (IHst _ _ _ eq_refl) as [s' ih <-].
+    exists (orelim s1 s2 s'). now constructor. now fsimpl.
+  - inv s... inv x. inv s1... inv x. asimpl.
+    eexists. now apply step_caseL. now asimpl.
+  - inv s... inv x. inv s1... inv x.
+    eexists. now apply step_caseR. now asimpl.
+Qed.
+
+Lemma step_inst {m n} (f : fin m -> tm n) (s t : tm m) :
+  step s t -> step (subst_tm f s) (subst_tm f t).
+Proof.
+   intros st. revert n f.  induction st; intros ? f; cbn; try (constructor; eauto).
+  - apply step_beta'. now asimpl.
+  - apply step_caseL'. now asimpl.
+  - apply step_caseR'. now asimpl.
+Qed.
+
+(** ** Multi-step reduction *)
+Inductive mstep {n} (s : tm n) : tm n -> Prop :=
+| mstep_refl : mstep s s
+| mstep_step t u : mstep s t -> step t u -> mstep s u.
+Hint Resolve mstep_refl.
+
+Lemma mstep_trans {n} (s t u : tm n) : mstep s t -> mstep t u -> mstep s u.
+Proof. intros st tu. revert s st. induction tu; eauto using mstep_step. Qed.
+
+Lemma mstep_lam n A (s t : tm (S n)) :
+  mstep s t -> mstep (lam A s) (lam A t).
+Proof. induction 1; eauto using mstep_step, step_abs. Qed.
+
+Lemma mstep_app n (s1 s2 : tm n) (t1 t2 : tm n) :
+  mstep s1 s2 -> mstep t1 t2 -> mstep (app s1 t1) (app s2 t2).
+Proof with eauto using @mstep, @step.
+  intros ms. induction 1. induction ms... auto...
+Qed.
+
+Lemma mstep_inl n (s1 s2: tm n):
+  mstep s1 s2 -> mstep (inl s1) (inl s2).
+Proof.
+  induction 1; [apply mstep_refl|].
+  eapply mstep_step; eauto using mstep_refl, mstep_trans, step_inl.
+Qed.
+
+Lemma mstep_inr n (s1 s2: tm n):
+  mstep s1 s2 -> mstep (inr s1) (inr s2).
+Proof.
+  induction 1; [apply mstep_refl|].
+  eapply mstep_step; eauto using mstep_refl, mstep_trans, step_inr.
+Qed.
+
+Lemma mstep_orelim n (s1 s2 : tm n) (t1 t2: tm (S n)) u1 u2:
+  mstep s1 s2 -> mstep t1 t2 -> mstep u1 u2 -> mstep (orelim s1 t1 u1) (orelim s2 t2 u2).
+Proof.
+  intros H1 H2 H3.
+  apply mstep_trans with (t := orelim s2 t1 u1).
+  - induction H1; [eapply mstep_refl|].
+    eapply mstep_step; eauto using mstep_refl, mstep_trans, step_orelim.
+  - apply mstep_trans with (t := orelim s2 t2 u1).
+    + induction H2; [eapply mstep_refl|].
+      eapply mstep_step; eauto using mstep_refl, mstep_trans, step_orelimL.
+    + induction H3; [eapply mstep_refl|].
+    eapply mstep_step; eauto using mstep_refl, mstep_trans, step_orelimR.
+Qed.
+
+Lemma mstep_inst m n (f : fin m -> tm n) (s t : tm m) :
+  mstep s t -> mstep (s[f]) (t[f]).
+Proof. induction 1; eauto using mstep_step, step_inst. Qed.
+
+Lemma mstep_subst m n (f g : fin m -> tm n) (s t : tm m) :
+  mstep s t -> (forall i, mstep (f i) (g i)) ->
+  mstep (s[f]) (t[g]).
+Proof with eauto using @mstep, @step.
+  intros st fg. apply mstep_trans with (t0 := t[f]); [eauto using mstep_inst|].
+  clear s st. revert n f g fg.
+  induction t; eauto using mstep_app, mstep_inl, mstep_inr; intros; simpl.
+  - apply mstep_lam. apply IHt. intros [i|]; [|constructor].
+    + asimpl. cbn. unfold funcomp. substify. now apply mstep_inst.
+  - apply mstep_orelim; [now apply IHt1 |apply IHt2|apply IHt3].
+    + intros [i|]; [|constructor].
+      * asimpl. cbn. unfold funcomp. substify. now apply mstep_inst.
+    +  intros [i|]; [|constructor].
+      * asimpl. cbn. unfold funcomp. substify. now apply mstep_inst.
+Qed.
+
+Lemma mstep_beta n (s1 s2 : tm (S n)) (t1 t2 : tm n) :
+  mstep s1 s2 -> mstep t1 t2 ->
+  mstep (s1 [t1..]) (s2 [t2..]).
+Proof.
+  intros st1 st2. apply mstep_subst; [assumption|].
+  now intros [|].
+Qed.
