coq/well-scoped-sums/sn_inductive_2a.v
@@ -1,0 +1,76 @@
+Require Import stlc reduction sn_defs.
+
+Ltac invTm :=
+match goal with
+|[_ : var_tm _ = ren_tm ?R ?M' |- _] => inv M'; simpl in *; try congruence
+|[_ : lam _ _ = ren_tm ?R ?M' |- _] => inv M'; simpl in *; try congruence
+|[_ : app _ _ = ren_tm ?R ?M' |- _] => inv M'; simpl in *; try congruence
+|[H: lam _ _ = lam _ _ |- _] => inv H
+|[H: app _ _ = app _ _|- _] => inv H
+|[H: ids _ = ids _|- _] => inv H
+|[_ : inl _ = ren_tm ?R ?M' |- _] => inv M'; simpl in *; try congruence
+|[_ : inr _ = ren_tm ?R ?M' |- _] => inv M'; simpl in *; try congruence
+|[_ : orelim _ _ _  = ren_tm ?R ?M' |- _] => inv M'; simpl in *; try congruence
+|[H: inl _ = inl _ |- _] => inv H
+|[H: inr _ = inr _ |- _] => inv H
+|[H: orelim _ _  _ = orelim _ _ _ |- _] => inv H
+end.
+
+Hint Constructors SN SNe SNRed.
+
+Lemma anti_rename:
+  (forall n (M: tm n), SN M -> forall n' M' (R: fin n' -> fin n), M = ren_tm R M' -> SN M')
+ /\ (forall n (M: tm n), SNe M -> forall n' M' (R: fin n' -> fin n), M = ren_tm R M' -> SNe M')
+ /\ (forall n (M N: tm n), SNRed M N -> forall n' (R: fin n' -> fin n) M', M = ren_tm R M' -> exists N', N = ren_tm R N' /\ SNRed M' N').
+Proof.
+  apply SN_multind; intros; repeat invTm; asimpl in *; subst; eauto.
+  - destruct (H0 _ _ _ (eq_refl _)) as (M''&->&?).
+    eapply SRed; eauto.
+  - destruct M'; simpl in *; try congruence.
+    inv H; now constructor.
+  - exists (M'0_1 [M'0_2..]).
+    split. now asimpl. constructor; eauto.
+  - destruct (H0 _ _ _ (eq_refl (ren_tm R0 M'1))) as (N'&->&A2).
+    exists (app N' M'2). split; [reflexivity| now constructor].
+  - destruct (H0 _ _ _ (eq_refl (ren_tm R M'0_1))) as (N'&->&A2).
+    exists (orelim N' M'0_2 M'0_3). split; [reflexivity|now constructor].
+  - exists (M'2 [M'1..]). split.
+    + now asimpl.
+    + constructor; [| | | reflexivity].
+      * now eapply H0.
+      * now eapply H2.
+      * now eapply H4.
+  - exists (M'3 [M'1..]). split.
+    + now asimpl.
+    + constructor; [| | |reflexivity].
+      * now eapply H0.
+      * now eapply H2.
+      * now eapply H4.
+Qed.
+
+Lemma rename :
+  (forall n (M: tm n), SN M -> forall n' (R: fin n -> fin n'), SN (ren_tm R M))
+  /\   (forall n (M: tm n),  SNe M -> forall n' (R: fin n -> fin n'), SNe (ren_tm R M))
+  /\ (forall n (M N: tm n), SNRed M N -> forall n' (R: fin n -> fin n'), SNRed (ren_tm R M) (ren_tm R N)).
+Proof.
+  apply SN_multind; intros; asimpl in *; eauto.
+  - constructor.
+  - intros. subst. constructor. auto. now asimpl.
+  - intros. subst. constructor. auto. auto. auto. now asimpl.
+  - intros. subst. constructor. auto. auto. auto. now asimpl.
+Qed.
+
+Lemma ext_SN n (M: tm n) (p: fin n) :
+  SN (app M (var_tm p)) -> SN M.
+Proof.
+  intros H. remember (app M (var_tm p)) as Mp. revert M p HeqMp.
+  induction H; intros; subst.
+  - inv H. now constructor.
+  - inv HeqMp.
+  - inv HeqMp.
+  - inv HeqMp.
+  - inv H.
+    + apply SAbs. eapply anti_rename. exact H0.
+      instantiate (1 := p..). substify. now asimpl.
+    + eapply SRed. exact H. eapply IHSN. reflexivity.
+Qed.
