coq/well-scoped-sums/sn_inductive_2b.v
@@ -1,0 +1,151 @@
+Require Import stlc reduction sn_defs sn_inductive_2a.
+
+(** ** Logical Relation *)
+Inductive closure {n} (R:  tm n -> Prop) : tm n -> Prop :=
+|CRefl (M: tm n) : R M -> closure R M
+|CNeutral (M: tm n) : SNe M -> closure R M
+|CStep (M M': tm n) : closure R M' -> SNRed M M' -> closure R M.
+
+Fixpoint Red {n} (A : ty) : tm n -> Prop :=
+  match A with
+  | Base => fun s => SN s
+  | Fun A B => fun s =>
+      forall n' (S : fin n -> fin n') (t : tm n'), Red A t -> Red B (app (ren_tm S s) t)
+  | Plus A B => closure (fun M => (exists M', M = inl M' /\ Red A M') \/ (exists M', M = inr M' /\ Red B M'))
+  end.
+
+Definition RedS {n n'} (S: fin n -> tm n') (Gamma: fin n -> ty) :=
+  forall i, Red (Gamma i) (S i).
+
+Lemma rename_red m n (f : fin m -> fin n) (s : tm m) A :
+  Red A s -> Red A (ren_tm f s).
+Proof.
+  revert s. induction A as [| A B|A IHA B IHB]; intros s; cbn.
+  - intros H. now apply rename.
+  - intros H n' g t lt. asimpl.  now apply H.
+  - intros H. induction H.
+    + apply CRefl. destruct H as [(M'&->&H2)|(M'&->&H2)]; [left|right].
+      * exists (ren_tm f M'). split; [reflexivity|now apply IHA].
+      * exists (ren_tm f M'). split; [reflexivity|now apply IHB].
+    + eapply CNeutral. now apply rename.
+    + asimpl. eapply CStep with (M'0 := ren_tm f M').
+      * assumption.
+      * apply rename. assumption.
+Qed.
+
+Lemma cr A:
+  (forall n (M: tm n), Red A M -> SN M) /\ (forall n (M: tm n), SNe M -> Red A M) /\ (forall n (M M': tm n), SNRed M M' -> Red A M' -> Red A M).
+Proof.
+  induction A as [|A IHA B IHB| A IHA B IHB].
+  - repeat split; intros.
+    + assumption.
+    + now apply SNeu.
+    + now apply SRed with (M' := M').
+  - repeat split; intros.
+    + eapply anti_rename with (R := shift) (M := ren_tm shift M); [|reflexivity].
+      eapply ext_SN, IHB. cbn in H. apply H, IHA. apply SVar with (x:= var_zero).
+    + intros g' R N H'. apply IHB.
+      apply SApp. now apply rename. now intuition.
+    + intros g' R N rn. apply IHB with (M' := app (ren_tm R M') N).
+     * constructor. now apply rename.
+     * apply H0, rn.
+   - repeat split; intros.
+    + induction H.
+      * destruct H as [(M'&->&H2)|(M'&->&H2)].
+        -- apply SInl. now apply IHA.
+        -- apply SInr. now apply IHB.
+      * now constructor.
+      * now apply SRed with (M' := M').
+    + now apply CNeutral.
+    + simpl in H0.
+      eapply CStep with (M'0 := M'); assumption.
+Qed.
+
+
+Lemma red_var n (p: fin n) A:
+  Red A (var_tm p).
+Proof. apply cr, SVar. Qed.
+
+Hint Resolve red_var.
+
+Definition ctx n := fin n -> ty.
+Inductive has_type {n} (Gamma : ctx n) : tm n -> ty -> Prop :=
+| ty_var_tm (x : fin n) :
+    has_type Gamma (var_tm x) (Gamma x)
+| ty_abs (S1 S2 : ty) (M : tm (S n)) :
+    @has_type (S n) (S1 .: Gamma) M S2 ->
+    has_type Gamma (lam S1 M) (Fun S1 S2)
+| ty_app (T S : ty) (M N : tm n) :
+    has_type Gamma M (Fun T S) ->
+    has_type Gamma N T ->
+    has_type Gamma (app M N) S
+| ty_inl M A B: has_type Gamma M A -> has_type Gamma (inl M) (Plus A B)
+| ty_inr M A B: has_type Gamma M B -> has_type Gamma (inr M) (Plus A B)
+| ty_or M A B C N1 N2 : has_type Gamma M (Plus A B) -> @has_type (S n) (A .: Gamma) N1 C -> @has_type (S n) (B .: Gamma) N2 C -> has_type Gamma (orelim M N1 N2) C
+.
+
+Notation "Gamma |- M : T" := (has_type Gamma M T) (at level 20, M at level 99).
+
+Lemma RedUp n n' (xi : fin n -> tm n') Gamma A:
+  RedS xi Gamma -> RedS (up_tm_tm xi) (A .: Gamma).
+Proof.
+  intros H [|]; cbn; eauto.
+  - apply rename_red, H.
+Qed.
+
+Lemma main_lemma n (M: tm n)  A Gamma:
+  Gamma |- M : A ->  forall n' (S: fin n -> tm n'), RedS S Gamma  -> Red A (subst_tm S M).
+Proof.
+  induction 1; intros.
+  - cbn. apply H.
+  - intros m R N rn.
+    eapply cr.
+    + cbn. econstructor.
+      * eapply cr; eauto.
+      * reflexivity.
+    + asimpl. eapply IHhas_type. intros [|]; eauto.
+      * cbn. unfold funcomp. renamify. apply rename_red. eauto.
+  - cbn.  specialize (IHhas_type2 _ _ H1).
+    specialize (IHhas_type1  _ _ H1 n' id _ IHhas_type2).
+    asimpl in IHhas_type1. eauto.
+  - specialize (IHhas_type _ _ H0).
+    constructor. left. exists (subst_tm S M). split; [reflexivity|auto].
+  - specialize (IHhas_type _ _ H0).
+    constructor. right. exists (subst_tm S M). split; [reflexivity|auto].
+  - specialize (IHhas_type1 _ _ H2). simpl. remember (subst_tm S M) as M'. clear M H HeqM'.
+    induction IHhas_type1.
+    + destruct H as [(M'&->&H)|(M'&->&H)].
+      * eapply cr.
+        -- apply SCaseL; [| | |reflexivity].
+           ++ eapply cr; eauto.
+           ++ eapply cr; eauto using RedUp.
+           ++ eapply cr; eauto using RedUp.
+        -- asimpl. apply IHhas_type2. intros [|]; eauto.
+      * eapply cr.
+        -- apply SCaseR; [| | |reflexivity].
+           ++ eapply cr; eauto.
+           ++ eapply cr; eauto using RedUp.
+           ++ eapply cr; eauto using RedUp.
+        -- asimpl. apply IHhas_type3. intros [|]; eauto.
+    + apply cr.
+      constructor.
+      * assumption.
+      * eapply cr; eauto using RedUp.
+      * eapply cr; eauto using RedUp.
+    + intros. subst.
+      assert (Red (Plus A B) M') as Red_M' by apply IHhas_type1.
+      simpl.
+      eapply cr.
+      instantiate (1 := (orelim M' (subst_tm (up_tm_tm S) N1) (subst_tm (up_tm_tm S) N2))).
+      now constructor. assumption.
+Qed.
+
+Lemma id_red g Gamma: @RedS g g ids Gamma.
+Proof. intros i. now apply red_var. Qed.
+
+Lemma norm n (M: tm n) (A: ty) Gamma: Gamma |- M : A -> SN M.
+Proof.
+  intros C.
+  assert (H := main_lemma _ _ _ _ C _ _ (@id_red n Gamma)).
+  asimpl in H. now apply cr in H.
+Qed.
