coq/well-scoped-sums/sn_inductive_soundness_1a.v
@@ -1,0 +1,236 @@
+(** * Different Characterisations Strong Normalisation *)
+
+Require Import stlc reduction sn_defs Coq.Program.Equality.
+Set Implicit Arguments.
+Unset Strict Implicit.
+
+(** ** Closure Properties of sn *)
+Lemma sn_preimage {m n} (f : tm m -> tm n) (s : tm m) :
+  (forall t u, step t u -> step (f t) (f u)) ->
+  sn (f s) -> sn s.
+Proof.
+  intros H sns. dependent induction sns. apply snI. intros t st.
+  eapply H0; eauto.
+Qed.
+
+Lemma sn_appL {n} (s : tm n) (t : tm n) :
+  sn (app s t) -> sn s.
+Proof. apply (@sn_preimage _ _ (fun s => app s t)); eauto using @step. Qed.
+
+Lemma sn_subst_tm {m n} (f : fin m -> tm n) (s : tm m) :
+  sn (subst_tm f s) -> sn s.
+Proof. apply sn_preimage. apply step_inst. Qed.
+
+Lemma closed_lam {n}  (s : tm (S n)) A:
+  sn (lam A s) <-> sn s.
+Proof.
+  split.
+  - eapply sn_preimage. apply step_abs.
+  - induction 1 as [M H IH].
+    constructor. intros M' C. inv C. auto.
+Qed.
+
+Lemma closed_appR n (M: tm n) (N: tm n)  :
+  sn (app M N) -> sn N.
+Proof. eapply sn_preimage. apply step_appR. Qed.
+
+Lemma closed_inl n (M: tm n)  :
+  sn M -> sn (inl  M).
+Proof. induction 1 as [M H IH]. constructor. intros M' C. inv C. auto. Qed.
+
+Lemma closed_inr n (M: tm n)  :
+  sn M -> sn (inr M).
+Proof. induction 1 as [M H IH]. constructor. intros M' C. inv C. auto. Qed.
+
+Lemma closed_orelim n (M: tm n) (N1: tm (S n)) N2:
+  sn (orelim M N1 N2) -> sn M /\ sn N1 /\ sn N2.
+Proof.
+  intros H. split.
+  - revert H. apply sn_preimage with (f := fun x => orelim x N1 N2).
+    intros t t' H. now apply step_orelim.
+  - split.
+    + revert H. apply sn_preimage with (f := fun x => orelim M x N2).
+      intros. now apply step_orelimL.
+    + revert H. eapply sn_preimage. apply step_orelimR.
+Qed.
+
+(* Weak Head Reduction *)
+Inductive redsn : forall n,  tm n -> tm n -> Prop :=
+ | redsn_beta n A (M: tm (S n)) (N: tm n) : sn N -> redsn (app (lam A M) N) (subst_tm (N.:ids) M)
+ | redsn_app n (R R' : tm n) (M : tm n) : redsn R R' -> redsn (app R M) (app R' M)
+ | redsn_or n (M M' : tm n) (N1 : tm (S n)) N2: redsn M M' -> redsn (orelim M N1 N2) (orelim M' N1 N2)
+ | redsn_caseL n (s: tm n) t t' (u: tm (S n)) : sn s -> sn t -> sn u -> t' = (t[s..]) -> redsn (orelim (inl s) t u) t'
+| redsn_caseR n (s: tm n) (t: tm (S n)) u u': sn s -> sn t -> sn u -> u' = (u[s..]) ->  redsn (orelim (inr s) t u) u'.
+
+
+Lemma fundamental_backwards n (M: tm (S n)) (N: tm n) A :
+   sn N -> sn (subst_tm (N.: ids) M) -> sn (app (lam A M) N).
+Proof.
+  intros sn_N sn_M'.
+  assert (H: sn M) by (now apply sn_subst_tm in sn_M').
+  revert M H sn_M'. induction sn_N as [N sn_N IH_N].
+  induction 1 as [M sn_M IH_M]. intros H. constructor. intros M' C. inv C.
+  - constructor. intros M' H'. inv H. now apply H.
+  - inv C. rename b2 into M'. eapply IH_M. assumption.
+    eauto using sn_mstep, mstep_beta, mstep_step.
+  - eapply IH_N; eauto.
+    + now constructor.
+    + eauto using sn_mstep, mstep_beta, mstep_step.
+Qed.
+
+Lemma fundamental_backwards_orl n (s : tm n) (t: tm (S n)) (u: tm (S n)):
+   sn s -> sn u -> sn (t[s..]) -> sn (orelim (inl s) t u).
+Proof.
+  intros sn_s sn_u H. assert (H': sn t) by (now apply sn_subst_tm in H).
+  revert t H' u sn_u H.
+  induction sn_s as [s sn_s IHs].
+  induction 1 as [u sn_u IHu].
+  induction 1 as [t sn_t IHt].  intros H. constructor. intros s' D. inv D.
+  - inv D. apply IHs. assumption. now constructor. now constructor.
+    eauto using sn_mstep, mstep_beta, mstep_step.
+  - apply IHu; eauto. now constructor. eauto using sn_mstep, mstep_beta, mstep_step.
+  - eapply IHt; eauto.
+  - assumption.
+Qed.
+
+Lemma fundamental_backwards_orr n (s : tm n) (t: tm (S n)) (u: tm (S n)):
+   sn s -> sn t -> sn (u[s..]) -> sn (orelim (inr s) t u).
+Proof.
+  intros sn_s sn_t H. assert (H': sn u) by (now apply sn_subst_tm in H).
+  revert u H' t sn_t H.
+  induction sn_s as [s sn_s IHs].
+  induction 1 as [t sn_t IHt].
+  induction 1 as [u sn_u IHu].  intros H. constructor. intros s' D. inv D.
+  - inv D. apply IHs; eauto. now constructor. now constructor.
+    eauto using sn_mstep, mstep_beta, mstep_step.
+  - eapply IHu; eauto.
+  - eapply IHt; eauto.  now constructor. eauto using sn_mstep, mstep_beta, mstep_step.
+  - assumption.
+Qed.
+
+(* Neutral terms *)
+Fixpoint neutral n (M: tm n) :=
+  match M with
+  | var_tm x => True
+  | app  s t => neutral s
+  | orelim s t u => neutral s
+  | _ => False
+  end.
+
+Lemma neutral_preservation n (M N: tm n):
+  neutral  M -> step M N ->  neutral N.
+Proof. intros H. induction 1; simpl in *; intuition. Qed.
+
+Lemma sn_app_neutral n (N : tm n) :
+   sn N -> forall (M: tm n), neutral M -> sn M -> sn (app M N).
+Proof.
+  induction 1 as [N sn_N IH_N].
+  induction 2 as [M sn_M IH_M].
+  constructor. intros M' C. inv C.
+  - contradiction.
+  - eauto using neutral_preservation.
+  - eauto using snI.
+Qed.
+
+Lemma sn_case_neutral n (N1 : tm (S n)):
+  sn N1 -> forall N2,  sn N2 -> forall (M: tm n), sn M -> neutral M ->  sn (orelim M N1 N2).
+Proof.
+  induction 1 as [N1 snN1 IHN1].
+  induction 1 as [N2 snN2 IHN2].
+  induction 1 as [M snM IHM].
+  intros H. constructor. intros M' H'. inv H'.
+  * apply IHM. assumption. eapply neutral_preservation; eassumption.
+  * now apply IHN1.
+  * now apply IHN2.
+  * contradiction.
+  * contradiction.
+Qed.
+
+Lemma sn_confluence n (M: tm n):
+  forall M' M'', redsn M M' -> step M M'' -> M' = M'' \/ exists M''', redsn M'' M''' /\ mstep M' M'''.
+Proof.
+  induction M as [n x | n M IHM N IHN |n M IHM| n M IHM | n M IHM | n M IHM N1 IHN1 N2 IHN2]; intros M' M'' D E; inv D; inv E.
+  - now left.
+  - inv E. right. eexists. split.
+    + now constructor.
+    + apply mstep_inst. eauto using mstep_step.
+  - right. eexists. split. econstructor. inv H; eauto. apply mstep_beta; eauto using mstep_step.
+  - inv D.
+  - destruct (IHM _ _ D E) as [IH|(M''&IH1&IH2)].
+    + subst. now left.
+    + right. eexists. split.
+      * econstructor. eassumption.
+      * eapply mstep_app. assumption. constructor.
+  - right. eexists. split.
+    + constructor. eassumption.
+    + eapply mstep_app. constructor. eauto using mstep_step.
+  - destruct (IHM _ _ D E) as [-> | (M''&IH1&IH2)].
+    + now left.
+    + right. exists (orelim M'' N1 N2). split; [now constructor|].
+      eauto using mstep_orelim.
+  - right. exists (orelim M' t2 N2). split.
+    + now constructor.
+    + eauto using mstep_orelim, mstep_step.
+  - right. exists (orelim M' N1 u2). split.
+    * now constructor.
+    * eauto using mstep_orelim, mstep_step.
+  - inv D.
+  - inv D.
+  - inv E. right. exists (N1 [s2..]). split.
+    + constructor; auto. inv H. now apply H.
+    + apply mstep_beta; eauto using mstep_step.
+  - right. exists (t2[s..]). split.
+    + constructor; eauto. inv H0. now apply H0.
+    + apply mstep_beta; eauto using mstep_step.
+  - right.  exists (N1[s..]). split.
+    + constructor; auto. inv H1. now apply H1.
+    + constructor.
+  - now left.
+  - inv E. right. exists (N2 [s2..]).  split.
+    + constructor; auto. inv H. now apply H.
+    + apply mstep_beta; eauto using mstep_step.
+  - right. exists (N2[s..]).  split.
+    + constructor; auto. inv H0. now apply H0.
+    + constructor.
+  - right. exists (u2[s..]). split.
+    + constructor; auto. inv H1. now apply H1.
+    + apply mstep_beta; eauto using mstep_step.
+  - now left.
+Qed.
+
+Lemma redsn_backwards n (M M': tm n):
+ redsn M M' -> sn M' -> sn M.
+Proof.
+ induction 1 as [|n M M' N H IH|n M M' N1 N2 H IH|n s t t' u h1 h2 h3|n s t u u' h1 h2 h3].
+ - intros D. eapply fundamental_backwards; eauto.
+ - intros D. specialize (IH (sn_appL D)).
+   assert (sn_N: sn N) by (now apply closed_appR in D).
+   revert M IH M' D H.
+   induction sn_N as [N sn_N IH_N]. induction 1 as [M sn_M IH_M].
+   constructor. intros M_N C. inv C.
+   + inv H.
+   + destruct (sn_confluence H C) as [E|(M'''&C1&C2)].
+     * now subst.
+     * eapply IH_M with (M' := M'''); eauto.
+       eapply sn_mstep; [|eassumption]. eapply mstep_app; eauto.
+   + eapply IH_N; eauto.
+     * now constructor.
+     * inv D. apply H. now constructor.
+ - intros D.
+   destruct (closed_orelim D) as (D1%IH&D2&D3). clear IH.
+   revert N1 D2 N2 D3 M' H D.
+   induction D1 as [M snM IHM].
+   induction 1 as [N1 snN1 IHN1].
+   induction 1 as [N2 snN2 IHN2].
+   constructor. intros M'' E. inv E.
+   + destruct (sn_confluence H E) as [F|(M''&F1&F2)].
+     * now subst.
+     * apply IHM with (M' := M''); eauto. now constructor. now constructor.
+       eapply sn_mstep; [|eassumption]. eapply mstep_orelim; eauto.
+   + eapply IHN1; eauto. now constructor. inv D. apply H0. now constructor.
+   + eapply IHN2; eauto. inv D. eapply H0. now constructor.
+   + inv H.
+   + inv H.
+ - subst. intros H'. now apply fundamental_backwards_orl.
+ - subst. intros H'. now apply fundamental_backwards_orr.
+Qed.
