coq/well-scoped/sn_inductive_2b.v
@@ -1,0 +1,82 @@
+Require Import stlc reduction sn_defs sn_inductive_2a.
+
+(** ** Logical Relation *)
+Fixpoint Red {n} (A : ty) : tm n -> Prop :=
+  match A with
+  | Base => fun s => SN s
+  | Fun A B => fun s =>
+      forall n' (S : fin n -> fin n') (t : tm n'), Red A t -> Red B (app (ren_tm S s) t)
+  end.
+
+Definition RedS {n n'} (S: fin n -> tm n') (Gamma: fin n -> ty) :=
+  forall i, Red (Gamma i) (S i).
+
+Lemma rename_red m n (f : fin m -> fin n) (s : tm m) A :
+  Red A s -> Red A (ren_tm f s).
+Proof.
+  revert s. destruct A as [| A B]; intros s; cbn.
+  - intros H. now apply rename.
+  - intros H n' g t lt. asimpl.  now apply H.
+Qed.
+
+Lemma cr A:
+  (forall n (M: tm n), Red A M -> SN M) /\ (forall n (M: tm n), SNe M -> Red A M) /\ (forall n (M M': tm n), SNRed M M' -> Red A M' -> Red A M).
+Proof.
+  induction A as [|A IHA B IHB].
+  - repeat split; intros.
+    + assumption.
+    + now apply SNeu.
+    + now apply SRed with (M' := M').
+  - repeat split; intros.
+    + eapply anti_rename with (R := shift) (M := ren_tm shift M); [|reflexivity].
+      eapply ext_SN, IHB. cbn in H. apply H, IHA. apply SVar with (x:= var_zero).
+    + intros g' R N H'. apply IHB.
+      apply SApp. now apply rename. now intuition.
+    + intros g' R N rn. apply IHB with (M' := app (ren_tm R M') N).
+     * constructor. now apply rename.
+     * apply H0, rn.
+Qed.
+
+Lemma red_var n (p: fin n) A:
+  Red A (var_tm p).
+Proof. apply cr, SVar. Qed.
+
+Definition ctx n := fin n -> ty.
+Inductive has_type {n} (Gamma : ctx n) : tm n -> ty -> Prop :=
+| ty_var_tm (x : fin n) :
+    has_type Gamma (var_tm x) (Gamma x)
+| ty_abs (S1 S2 : ty) (M : tm (S n)) :
+    @has_type (S n) (S1 .: Gamma) M S2 ->
+    has_type Gamma (lam S1 M) (Fun S1 S2)
+| ty_app (T S : ty) (M N : tm n) :
+    has_type Gamma M (Fun T S) ->
+    has_type Gamma N T ->
+    has_type Gamma (app M N) S.
+Notation "Gamma |- M : T" := (has_type Gamma M T) (at level 20, M at level 99).
+
+Lemma main_lemma n (M: tm n)  A Gamma:
+  Gamma |- M : A ->  forall n' (S: fin n -> tm n'), RedS S Gamma  -> Red A (subst_tm S M).
+Proof.
+  induction 1; intros.
+  - cbn. apply H.
+    - intros m R N rn.
+    eapply cr.
+    + cbn. econstructor.
+      * eapply cr; eauto.
+      * reflexivity.
+    + asimpl. eapply IHhas_type. intros [|]; eauto.
+      * cbn. unfold funcomp. renamify. apply rename_red. eauto.
+  - cbn.  specialize (IHhas_type2 _ _ H1).
+    specialize (IHhas_type1  _ _ H1 n' id _ IHhas_type2).
+    asimpl in IHhas_type1. eauto.
+Qed.
+
+Lemma id_red g Gamma: @RedS g g ids Gamma.
+Proof. intros i. now apply red_var. Qed.
+
+Lemma norm n (M: tm n) (A: ty) Gamma: Gamma |- M : A -> SN M.
+Proof.
+  intros C.
+  assert (H := main_lemma _ _ _ _ C _ _ (@id_red n Gamma)).
+  asimpl in H. now apply cr in H.
+Qed.
