coq/well-scoped/depgraph.v
@@ -1,7 +1,0 @@
-Require dpdgraph.dpdgraph.
-
-Require sn.
-Require axioms.
-Print FileDependGraph sn.Reduction sn.ManyStepReduction sn.Reduction sn.L sn.SN sn.Typing axioms.
-
-Print FileDependGraph sn.
